def

definitions.v
@@ -14,7 +14,7 @@ Inductive trm : Set :=
    k is the current depth *)
 Fixpoint open_rec (k : nat) (x : var) (t : trm) : trm :=
   match t with
-    | trm_bvar i    => if (beq_nat k i) then trm_fvar x else (trm_bvar i)
+    | trm_bvar i    => if (eq_nat_dec k i) then trm_fvar x else (trm_bvar i)
     | trm_fvar y    => trm_fvar y 
     | trm_app t1 t2 => trm_app (open_rec k x t1) (open_rec k x t2)
     | trm_abs t1    => trm_abs (open_rec (S k) x t1) 
@@ -26,7 +26,7 @@ Definition open t x := open_rec 0 x t.
 Fixpoint close_var_rec (k : nat) (x : var) (t : trm) : trm :=
   match t with
     | trm_bvar i    => trm_bvar i 
-    | trm_fvar y    => if beq_nat x y then (trm_bvar k) else (trm_fvar y)
+    | trm_fvar y    => if eq_nat_dec x y then (trm_bvar k) else (trm_fvar y)
     | trm_app t1 t2 => trm_app (close_var_rec k x t1) (close_var_rec k x t2)
     | trm_abs t1    => trm_abs (close_var_rec (S k) x t1) 
   end.
@@ -44,7 +44,7 @@ Fixpoint locally_closed_at_rec (k : nat) (t : trm) : Prop :=
 Definition locally_closed (t:trm) : Prop := locally_closed_at_rec 0 t.
 
 Fixpoint free_variables (t:trm) : list var :=
-   match t with
+  match t with
     | trm_bvar i    => nil
     | trm_fvar x    => x :: nil
     | trm_app t1 t2 => (free_variables t1)++(free_variables t2)
@@ -57,90 +57,353 @@ Definition fresh (x:var) (t:trm) : Prop :=
 Definition closed (t:trm) : Prop :=
   (free_variables t) = nil.
 
-Lemma open_var_fv:
-  forall x:var, forall t:trm,  incl (free_variables (open t x)) (x::(free_variables t)).
+Lemma close_open_var_rec :
+  forall t:trm, forall u:var,forall k:nat, fresh u t -> (close_var_rec k u (open_rec k u t)) = t.
 Proof.
- intros.
- unfold incl.
- intro.
- induction t.
- simpl.
- unfold open.
- unfold open_rec.
- induction n.
- simpl.
- intro. 
- exact H.
- simpl.
- right.
- exact H.
- simpl.
- right.
- exact H.
- simpl. 
- intro. 
- right.
- apply in_app_or in H.
- unfold open in IHt1.
- unfold open in IHt2.
- destruct H.
- apply IHt1 in H.
- apply in_or_app.
- left.
- apply in_cons.
-
- inversion H.
- rewrite H0 in H.
- 
- 
- simpl.
- 
- apply in_cons with (a:=x) in H .
- 
+  intros t u.
+  induction t.
+  intro k.
+  unfold fresh.
+  unfold free_variables.
+  unfold close_var_rec.
+  unfold open_rec.
+  intro.
+  destruct (eq_nat_dec k n).
+  destruct (eq_nat_dec u u).
+  rewrite e.
+  reflexivity.
+  contradict n0.
+  reflexivity.
+  reflexivity.
+  destruct (eq_nat_dec u v).
+  rewrite e.
+  simpl.
+  unfold fresh.
+  unfold free_variables.
+  intros.  
+  contradict H.
+  simpl.
+  left.
+  reflexivity.
+  unfold fresh.
+  unfold free_variables.
+  simpl.
+  intros.
+  destruct (eq_nat_dec u v).
+  contradict H.
+  left.
+  rewrite e.
+  reflexivity.
+  reflexivity.
+  intros.
+  unfold fresh  in *.
+  simpl.
+  rewrite IHt1.
+  rewrite IHt2.
+  reflexivity.  
+  contradict H.
+  simpl.
+  SearchPattern ( In _ ( _ ++ _ )).  
+  apply in_or_app.
+  right.
+  exact H.
+  simpl in H.
+  contradict H.
+  apply in_or_app.
+  left.
+  exact H.
+  intros.
+  simpl.
+  unfold fresh in H.
+  unfold fresh in IHt.
+  simpl in H.
+  rewrite IHt.
+  reflexivity.
+  exact H.
 
 Qed.
 
-Lemma close_var_fv:
-  forall x:var, forall t:trm,  incl (free_variables (close_var x t)) (x (free_variables t)).
-Proof.
-
-
-Qed.
-
-Lemma lc_at_app:
-  forall c:nat, forall t1:trm, forall t2:trm, locally_closed_at_rec c (trm_app t1 t2) -> (locally_closed_at_rec c t1) /\ (locally_closed_at_rec c t2).
+Lemma close_open_var :
+  forall t:trm, forall u:var, 
+    fresh u t -> (close_var u (open t u)) = t.
 Proof.
   intros.
-  simpl in H.
+  apply close_open_var_rec.
   exact H.
 Qed.
 
+Lemma incl_nil : 
+  forall (A : Set) (l : list A), incl nil l.
+Proof.
+  intros A l.
+  unfold incl in |- *.
+  unfold In in |- *; contradiction.
+Qed.
+
+
+Lemma elim_incl_cons : forall (A : Type) (x : A) (xs zs : list A),
+                         incl (x :: xs) zs ->
+                         In x zs /\ incl xs zs.
+Proof. unfold incl. auto with datatypes. Qed.
 
 
 
+Lemma elim_incl_app : forall (A : Type) (xs ys zs : list A),
+                        incl (xs ++ ys) zs ->
+                        incl xs zs /\ incl ys zs.
+Proof. unfold incl. auto with datatypes. Qed.
 
-Lemma close_open_var :
-  forall t:trm, forall k:nat, exists u:var, fresh u t -> (close_var_rec k u (open_rec k u t)) = t.
+
+Lemma incl_app_comm :
+  forall (A : Type) (x:A) (xs ys zs : list A),
+    incl xs (x::ys++zs) ->  incl xs (x::zs++ys).
+Proof.
+  intros A x xs ys zs.
+  unfold incl. 
+  intros.
+  apply in_inv with (b:=a) in H.
+  rewrite app_comm_cons.
+  apply in_or_app.
+  
+  elim H.
+  intro.
+  rewrite H1.
+  simpl.
+  left.  
+  left.  
+  reflexivity.
+  intro.
+  apply in_app_or in H1.
+  elim H1.
+  intro.
+  right.
+  exact H2.
+  intro.
+  left.
+  apply in_cons.
+  exact H2.
+  exact H0.
+Qed.
+
+
+Lemma open_var_fv:
+  forall x:var, forall t:trm, forall k:nat, incl (free_variables (open_rec k x t)) (x::(free_variables t)).
+Proof.
+  intros x t.
+  
+
+
+  induction t.
+  simpl.
+  intro k.
+  destruct (eq_nat_dec k n).
+  simpl.
+  SearchPattern (incl _ _ ).
+
+  apply incl_refl.
+  simpl.
+  apply incl_nil.
+  intro k.
+  simpl.
+  apply incl_tl.
+  apply incl_refl.
+  intro k.
+  simpl.
+  apply incl_app.
+
+  rewrite app_comm_cons.
+  apply incl_appl.
+  apply IHt1.
+  apply incl_app_comm.
+  rewrite app_comm_cons.
+  apply incl_appl.
+  apply IHt2.
+
+  simpl.
+  intro k.
+  apply IHt.
+Qed.
+
+
+Fixpoint remove_var (x:var) (l:list var) : list var :=
+  match l with
+  | nil => nil
+  | h::tl => if (eq_nat_dec x h) then remove_var x tl else h::(remove_var x tl) 
+  end.
+
+Lemma remove_cons:
+  forall (x:var) (l1:list var) (l2:list var),
+    (remove_var x (l1++l2)) = (remove_var x l1)++(remove_var x l2).
+Proof.
+  intros.
+  induction l1.
+  - simpl. 
+    reflexivity.
+  - induction l2.
+    * simpl.
+      remember (eq_nat_dec x a) as cond.
+      simpl in IHl1.
+      rewrite IHl1.
+      induction cond.
+      + reflexivity.
+      + simpl.
+        reflexivity.
+    * simpl.
+      remember (eq_nat_dec x a) as cond1.
+      induction cond1. 
+      Admitted.
+
+
+
+Lemma fv_abs:
+  forall t:trm, 
+    free_variables t = free_variables (trm_abs t).
+Proof.
+  intros.
+  simpl.
+  reflexivity.
+Qed.
+
+Lemma close_var_fv:
+  forall (x:var), forall (t:trm),
+    (free_variables (close_var x t)) = (remove_var x (free_variables t)).
 Proof.
   intros.
   induction t.
-  - induction k.
+  - simpl.
+    reflexivity.
     
+  - unfold close_var.
+    simpl.
+    remember (eq_nat_dec x v) as e. 
+    induction e.
+    * simpl. 
+      reflexivity.
+    * simpl.
+      reflexivity.
 
-Qed.
+  - simpl.
+    rewrite remove_cons.
+    inversion IHt1.
+    inversion IHt2.
+    unfold close_var.
+    reflexivity.
 
-Lemma open_close_var :
-  forall u:var, forall t:trm, (open_rec 0 u (close_var_rec 0 u t)) = t.
+  - 
+
+
+
+
+
+
+
+Fixpoint subst (x:var) (u:trm) (t:trm) : trm :=
+  match t with
+    | trm_bvar i    => trm_bvar i
+    | trm_fvar y    => if (eq_nat_dec x y) then u else trm_fvar y 
+    | trm_app t1 t2 =>  trm_app (subst x u t1) (subst x u t2)
+    | trm_abs t1    =>  trm_abs (subst x u t1)
+  end.
+
+
+Lemma subst_lc :
+  forall (t:trm) (u:trm) (x:var) (k:nat),
+    locally_closed_at_rec k t /\ locally_closed_at_rec k u -> locally_closed_at_rec k (subst x u t).
 Proof.
-  intros.
+(*   intros t u x. *)
+(*   induction t. *)
+
+(*   simpl. *)
+(*   intros. *)
+(*   elim H. *)
+(*   intros. *)
+(*   exact H0. *)
+(*   unfold subst. *)
+(*   simpl. *)
+(*   intros.   *)
+(*   destruct (eq_nat_dec x v). *)
+(*   elim H. *)
+(*   intros. *)
+(*   exact H1. *)
+(*   simpl. *)
+(*   reflexivity. *)
   
-Qed.
+(*   intros. *)
+(*   simpl. *)
 
-Definition locally_closed t := locally_closed_rec 0 t.
+(*   simpl in H. *)
+(*   elim H. *)
+(*   intros. *)
+(*   elim H0. *)
+(*   intros. *)
+(*   split. *)
+(*   apply IHt1. *)
+(*   split. *)
+(*   exact H2. *)
+(*   exact H1. *)
+(*   apply IHt2. *)
+(*   split. *)
+(*   exact H3. *)
+(*   exact H1. *)
+  (* induction u. *)
+  
+  (* simpl. *)
+  (* intros. *)
+  (* apply IHt.  *)
+  (* elim H. *)
+  (* intros. *)
+  (* split. *)
+  (* exact H0. *)
+  (* simpl. *)
+  (* SearchPattern ( _ < S _ ). *)
+  (* apply lt_S. *)
+  (* exact H1. *)
+  
+  (* intros. *)
+  (* simpl. *)
+  (* apply IHt. *)
+  (* split. *)
+  (* elim H. *)
+  (* intros. *)
+  (* simpl in *. *)
+  (* exact H0. *)
+  (* elim H. *)
+  (* intros. *)
+  (* simpl in *. *)
+  (* reflexivity. *)
 
-Example closed_ex1:
-  locally_closed (trm_abs (trm_bvar 0)).
-Proof.
-  compute. reflexivity.
-Qed.
+  (* simpl in *. *)
+  (* intros. *)
+  (* apply IHt.   *)
+  (* split. *)
+  (* elim H. *)
+  (* intros. *)
+  (* exact H0. *)
+  (* simpl. *)
+  (* split. *)
+  (* elim H. *)
+  (* simpl in *. *)
+  (* intros.   *)
+  (* elim H1. *)
+  (* intros. *)
+  Admitted.
+
+
+
+Lemma subst_open_var : 
+  forall (x:var) (y:var) (u:trm) (t:trm), forall (k:nat),
+    x <> y -> locally_closed_at_rec k u -> subst x u (open_rec k x t) = open_rec k y (subst x u t).
+Proof. 
+  Admitted.
+
+
+
+
+
+Lemma subst_close_var : 
+  forall (x:var) (y:var) (u:trm) (t:trm), forall (k:nat),
+    x <> y -> fresh k u -> subst x u (close_var_rec k x t) = close_var_rec k y (subst x u t).
+Proof. 
+  Admitted.
+
 
